Applied the idea of dropping branch predictors; fixed some bugs in the processor.

processors/Decode.v
@@ -196,11 +196,58 @@ Section Processor.
           Retv
       }.
 
+    Definition decodeNondet :=
+      MODULE {
+        Rule "doDecode" :=
+          Call i2d <- i2dDeq();
+          LET f2d <- #i2d!I2D@."f2dOrig";
+          LET pc <- #f2d!(F2D addrSize)@."pc";
+          LET instStr <- #i2d!I2D@."iMemRep";
+          LET inst <- #instStr!(RsToProc dataBytes)@."data";
+
+          Call decEpoch <- decGetEpoch2();
+          Call exeEpoch <- exeGetEpoch2();
+
+          If (#exeEpoch == #f2d!(F2D addrSize)@."exeEpoch"
+              && #decEpoch == #f2d!(F2D addrSize)@."decEpoch")
+          then
+            LET predPc <- #f2d!(F2D addrSize)@."predPc";
+            LET dInst <- decodeInst _ inst;
+            LET iType <- #dInst!DecodedInst@."iType";
+            
+            If (#iType != $$iTypeUnsupported)
+            then
+              (* Value bypassing related, may have some other iType's that need registration *)
+              If (#dInst!DecodedInst@."hasDst")
+              then
+                If (#iType == $$iTypeLd)
+                then
+                  Call bpRegisterM(#dInst!DecodedInst@."dst");
+                  Retv
+                else
+                  Call bpRegisterE(#dInst!DecodedInst@."dst");
+                  Retv;
+                Retv;
+
+              Nondet predPcN : SyntaxKind (Bit addrSize);
+
+              Call (redirSetValid addrSize "dec")(
+                     STRUCT { "pc" ::= #pc;
+                              "nextPc" ::= #predPcN });
+              Call d2rEnq(STRUCT { "pc" ::= #pc;
+                                   "predPc" ::= #predPcN;
+                                   "dInst" ::= #dInst;
+                                   "exeEpoch" ::= #exeEpoch });
+              Retv;
+            Retv;
+          Retv
+      }.
+    
   End Decode.
 
 End Processor.
 
-Hint Unfold bht bhtTrain decode : ModuleDefs.
+Hint Unfold bht bhtTrain decode decodeNondet : ModuleDefs.
 
 Hint Unfold satCntInit getIndex getTaken nextSatCnt bhtUpdateStr
      bhtPredTaken bhtUpdate bhtTrainDeq
@@ -222,6 +269,10 @@ Section Wf.
     forall i2dName d2rName, ModPhoasWf (decode addrSize i2dName d2rName decodeInst).
   Proof. kequiv. Qed.
 
+  Lemma decodeNondet_ModEquiv:
+    forall i2dName d2rName, ModPhoasWf (decodeNondet addrSize i2dName d2rName decodeInst).
+  Proof. kequiv. Qed.
+
   Lemma bht_ModRegsWf:
     ModRegsWf (bht addrSize indexSize).
   Proof. kvr. Qed.
@@ -234,8 +285,12 @@ Section Wf.
     forall i2dName d2rName, ModRegsWf (decode addrSize i2dName d2rName decodeInst).
   Proof. kvr. Qed.
 
+  Lemma decodeNondet_ModRegsWf:
+    forall i2dName d2rName, ModRegsWf (decodeNondet addrSize i2dName d2rName decodeInst).
+  Proof. kvr. Qed.
+
 End Wf.
 
-Hint Resolve bht_ModEquiv bhtTrain_ModEquiv decode_ModEquiv.
-Hint Resolve bht_ModRegsWf bhtTrain_ModRegsWf decode_ModRegsWf.
+Hint Resolve bht_ModEquiv bhtTrain_ModEquiv decode_ModEquiv decodeNondet_ModEquiv.
+Hint Resolve bht_ModRegsWf bhtTrain_ModRegsWf decode_ModRegsWf decodeNondet_ModRegsWf.
 
