processors/InOrderEightStage.v
@@ -24,6 +24,8 @@ Section Processor.
   Definition decName := "dec".
   Definition exeName := "exe".
   Definition bhtTrainName := "bhtTrain".
+
+  (** TODO: need to differentiate below interfaces to memory *)
   Definition iExecName := "exec".
   Definition dExecName := "exec".
 
@@ -35,35 +37,36 @@ Section Processor.
   Definition btb := btb btbIndexSize btbTagSize Hbtb.
   Definition decRedir := redirect addrSize decName.
   Definition exeRedir := redirect addrSize exeName.
-  Definition f2i := @nativeFifo f2iName (Struct (F2I addrSize dataBytes)) Default.
+  Definition f2i := @nativeSimpleFifo f2iName (Struct (F2I addrSize dataBytes)) Default.
 
   (** IMem related *)
   Definition iMem := iMem addrSize dataBytes f2iName i2dName iExecName.
-  Definition i2d := @nativeFifo i2dName (Struct (I2D addrSize dataBytes)) Default.
+  Definition i2d := @nativeSimpleFifo i2dName (Struct (I2D addrSize dataBytes)) Default.
 
   (** Decode related *)
   Definition decode := decode addrSize i2dName d2rName decodeInst.
   Definition bht := bht addrSize bhtIndexSize.
-  Definition bhtTrain := fifo bhtTrainName bhtTrainSize (Struct (bhtUpdateStr addrSize)).
-  Definition d2r := @nativeFifo d2rName (Struct (D2R addrSize dataBytes rfIdx)) Default.
+  Definition bhtTrain := bhtTrain addrSize bhtTrainName.
+  Definition bhtTrainQ := simpleFifo bhtTrainName bhtTrainSize (Struct (bhtUpdateStr addrSize)).
+  Definition d2r := @nativeSimpleFifo d2rName (Struct (D2R addrSize dataBytes rfIdx)) Default.
 
   (** RegRead related *)
   Definition regRead := regRead addrSize dataBytes rfIdx d2rName r2eName.
   Definition rf := regFile dataBytes rfIdx.
   Definition bypass := bypass dataBytes rfIdx.
-  Definition r2e := @nativeFifo r2eName (Struct (R2E addrSize dataBytes rfIdx)) Default.
+  Definition r2e := @nativeSimpleFifo r2eName (Struct (R2E addrSize dataBytes rfIdx)) Default.
 
   (** Execute related *)
   Definition execute := execute r2eName e2mName bhtTrainName execInst.
-  Definition e2m := @nativeFifo e2mName (Struct (E2M addrSize dataBytes rfIdx)) Default.
+  Definition e2m := @nativeSimpleFifo e2mName (Struct (E2M addrSize dataBytes rfIdx)) Default.
 
   (** Mem related *)
   Definition mem := mem addrSize dataBytes rfIdx e2mName m2dName.
-  Definition m2d := @nativeFifo m2dName (Struct (M2D addrSize dataBytes rfIdx)) Default.
+  Definition m2d := @nativeSimpleFifo m2dName (Struct (M2D addrSize dataBytes rfIdx)) Default.
 
   (** DMem related *)
   Definition dMem := dMem addrSize dataBytes rfIdx m2dName d2wName dExecName.
-  Definition d2w := @nativeFifo d2wName (Struct (D2W addrSize dataBytes rfIdx)) Default.
+  Definition d2w := @nativeSimpleFifo d2wName (Struct (D2W addrSize dataBytes rfIdx)) Default.
 
   (** Writeback related *)
   Definition writeback := writeback addrSize dataBytes rfIdx d2wName.
@@ -71,7 +74,7 @@ Section Processor.
   Definition inOrderEight :=
     (fetch ++ btb ++ decRedir ++ exeRedir ++ decEpoch ++ exeEpoch ++ f2i ++
            iMem ++ i2d ++
-           decode ++ bht ++ bhtTrain ++ d2r ++
+           decode ++ bht ++ bhtTrain ++ bhtTrainQ ++ d2r ++
            regRead ++ rf ++ bypass ++ r2e ++
            execute ++ e2m ++
            mem ++ m2d ++
