refinements/DropBranchPredictors.v
@@ -1,0 +1,118 @@
+Require Import Kami.
+Require Import Lib.CommonTactics Lib.Indexer.
+Require Import Kami.Decomposition.
+Require Import Ex.MemTypes Ex.OneEltFifo.
+Require Import Proc.AbstractIsa Proc.Fetch Proc.Decode Proc.Execute Proc.InOrderEightStage.
+
+Set Implicit Arguments.
+Open Scope string.
+
+Section Processor.
+  Variables addrSize dataBytes rfIdx: nat.
+
+  Variable decodeInst: DecodeT dataBytes rfIdx.
+  Variable execInst: ExecT addrSize dataBytes rfIdx.
+
+  Variables btbIndexSize btbTagSize bhtIndexSize bhtTrainSize: nat.
+  Hypothesis (Hbtb: btbIndexSize + btbTagSize = addrSize).
+
+  (** Fetch related *)
+  Definition fetchNondet := fetchNondet addrSize dataBytes f2iName.
+  Definition decRedir := decRedir addrSize.
+  Definition exeRedir := exeRedir addrSize.
+  Definition f2i := f2i addrSize dataBytes.
+
+  (** IMem related *)
+  Definition iMem := iMem addrSize dataBytes.
+  Definition i2d := i2d addrSize dataBytes.
+
+  (** Decode related *)
+  Definition decodeNondet := decodeNondet addrSize i2dName d2rName decodeInst.
+  Definition d2r := d2r addrSize dataBytes rfIdx.
+
+  (** RegRead related *)
+  Definition regRead := regRead addrSize dataBytes rfIdx.
+  Definition rf := rf dataBytes rfIdx.
+  Definition bypass := bypass dataBytes rfIdx.
+  Definition r2e := r2e addrSize dataBytes rfIdx.
+
+  (** Execute related *)
+  Definition executeNondet := executeNondet r2eName e2mName execInst.
+  Definition e2m := e2m addrSize dataBytes rfIdx.
+
+  (** Mem related *)
+  Definition mem := mem addrSize dataBytes rfIdx.
+  Definition m2d := m2d addrSize dataBytes rfIdx.
+
+  (** DMem related *)
+  Definition dMem := dMem addrSize dataBytes rfIdx.
+  Definition d2w := d2w addrSize dataBytes rfIdx.
+
+  (** Writeback related *)
+  Definition writeback := writeback addrSize dataBytes rfIdx.
+
+  (* inOrderEight :=
+     (fetch ++ btb ++ decRedir ++ exeRedir ++ decEpoch ++ exeEpoch ++ f2i ++
+     iMem ++ i2d ++
+     decode ++ bht ++ bhtTrain ++ bhtTrainQ ++ d2r ++
+     regRead ++ rf ++ bypass ++ r2e ++
+     execute ++ e2m ++
+     mem ++ m2d ++
+     dMem ++ d2w ++
+     writeback)%kami.
+   *)
+  Definition inOrderEight :=
+    inOrderEight decodeInst execInst
+                 btbIndexSize btbTagSize bhtIndexSize bhtTrainSize
+                 Hbtb.
+
+  Definition inOrderEight0 :=
+    (fetchNondet ++ decRedir ++ exeRedir ++ decEpoch ++ exeEpoch ++ f2i ++
+                 iMem ++ i2d ++
+                 decodeNondet ++ d2r ++
+                 regRead ++ rf ++ bypass ++ r2e ++
+                 executeNondet ++ e2m ++
+                 mem ++ m2d ++
+                 dMem ++ d2w ++
+                 writeback)%kami.
+
+  Section Refinement.
+
+    (* Eval compute in (Struct.namesOf (getRegInits inOrderEight)). *)
+    (* Eval compute in (Struct.namesOf (getRegInits inOrderEight0)). *)
+
+    Local Definition dropRegs : list string :=
+      ["full.bhtTrain"; "empty.bhtTrain"; "deqP.bhtTrain"; "enqP.bhtTrain"; "elt.bhtTrain";
+         "satCnt"; "btbValid"; "btbTags"; "btbTargets"].
+
+    Local Definition theta (s: RegsT) : RegsT := M.complement s dropRegs.
+
+    (* Eval compute in (getDefs inOrderEight). *)
+    (* Eval compute in (getDefs inOrderEight0). *)
+
+    Local Definition dropMeths : list string :=
+      ["firstElt.bhtTrain"; "deq.bhtTrain"; "enq.bhtTrain"; "update"; "predTaken";
+         "btbUpdate"; "btbPredPc"].
+    (* pose (getDefs inOrderEight) as pdefs; compute in pdefs. *)
+    (* pose (getDefs inOrderEight0) as ndefs; compute in ndefs. *)
+    (* pose (fold_left (fun nl e => *)
+    (*                    if in_dec string_dec e ndefs then nl else e :: nl) pdefs nil) as ddefs. *)
+    (* compute in ddefs. *)
+
+    Local Definition p (n: string) (v: (sigT SignT)): option (sigT SignT) :=
+      if in_dec string_dec n dropMeths
+      then None
+      else Some v.
+
+    Local Definition ruleMap (o: RegsT) (n: string) : option string := Some n.
+    
+    Theorem inOrderEight_inOrderEight0: inOrderEight <<== inOrderEight0.
+    Proof.
+      (* apply traceRefines_labelMap_weakening with (vp:= p); [kequiv| |]. *)
+      (* apply decompositionDrop with (theta:= theta) (ruleMap:= ruleMap). *)
+    Admitted.
+
+  End Refinement.
+  
+End Processor.
+
